Merged, with some sorrys

vipersemabstract/Instantiation.thy
@@ -251,9 +251,13 @@ definition make_semantic_assertion :: "('a, 'a virtual_state) interp \<Rightarro
   "make_semantic_assertion \<Delta> F A \<omega> \<longleftrightarrow> \<omega> \<in> (\<langle>\<Delta>, F\<rangle> \<Turnstile> \<langle>A\<rangle>)"
 *)
 
+
+
+
+(*
 definition make_semantic_assertion :: "('a, 'a virtual_state) interp \<Rightarrow> (pure_exp, pure_exp atomic_assert) assert \<Rightarrow> 'a equi_state set" where
   "make_semantic_assertion \<Delta> A = { \<omega> |\<omega>. \<Delta> \<Turnstile> \<langle>A; \<omega>\<rangle> }"
-
+*)
 
 fun make_semantic_vtyp :: "('a, 'a virtual_state) interp \<Rightarrow> vtyp \<Rightarrow> 'a val abs_vtyp" where
   "make_semantic_vtyp _ TInt = { VInt n |n. True }"
@@ -272,34 +276,6 @@ datatype 'a custom =
   FieldAssign "('a equi_state, address) exp" field_ident "('a equi_state, 'a val) exp"
   | Label label
 
-fun compile :: "('a, 'a virtual_state) interp \<Rightarrow> stmt \<Rightarrow> ('a equi_state, 'a val, 'a custom) abs_stmt"
-  where
-  "compile \<Delta> stmt.Skip = abs_stmt.Skip"
-
-| "compile \<Delta> (stmt.If b C1 C2) = abs_stmt.If (make_semantic_bexp \<Delta> b) (compile \<Delta> C1) (compile \<Delta> C2)"
-| "compile \<Delta> (stmt.Seq C1 C2) = abs_stmt.Seq (compile \<Delta> C1) (compile \<Delta> C2)"
-
-| "compile \<Delta> (stmt.Havoc x) = abs_stmt.Havoc x"
-| "compile \<Delta> (stmt.LocalAssign x e) = abs_stmt.LocalAssign x (make_semantic_exp \<Delta> e)"
-
-
-| "compile \<Delta> (stmt.Inhale A) = abs_stmt.Inhale (make_semantic_assertion \<Delta> A)"
-| "compile \<Delta> (stmt.Exhale A) = abs_stmt.Exhale (make_semantic_assertion \<Delta> A)"
-| "compile \<Delta> (stmt.Assert A) = abs_stmt.Assert (make_semantic_assertion \<Delta> A)"
-| "compile \<Delta> (stmt.Assume A) = abs_stmt.Assume (make_semantic_assertion \<Delta> A)"
-
-| "compile \<Delta> (stmt.Unfold _ _ _) = abs_stmt.Skip"
-| "compile \<Delta> (stmt.Fold _ _ _) = abs_stmt.Skip"
-| "compile \<Delta> (stmt.Package _ _) = abs_stmt.Skip"
-| "compile \<Delta> (stmt.Apply _ _) = abs_stmt.Skip"
-
-(* TODO: We can take the program as input, and emit the encodings *)
-| "compile \<Delta> (stmt.MethodCall _ _ _) = undefined"
-| "compile \<Delta> (stmt.While b I C) = undefined"
-| "compile \<Delta> (stmt.Scope _ _) = undefined"
-
-| "compile \<Delta> (stmt.FieldAssign r f e) = abs_stmt.Custom (FieldAssign (make_semantic_rexp \<Delta> r) f (make_semantic_exp \<Delta> e))"
-| "compile \<Delta> (stmt.Label l) = abs_stmt.Custom (Label l)"
 
 
 
@@ -1169,10 +1145,53 @@ proof
 
 qed
 
-definition viper_prog_verifies where
-  "viper_prog_verifies Pr \<Delta> ty C \<omega> \<longleftrightarrow> ConcreteSemantics.verifies ty (compile \<Delta> C) \<omega>"
-  (* ty is a type-context *)
 
+definition make_semantic_assertion :: "('a, 'a virtual_state) interp \<Rightarrow> (field_name \<rightharpoonup> vtyp) \<Rightarrow> (pure_exp, pure_exp atomic_assert) assert \<Rightarrow> 'a equi_state set" where
+  "make_semantic_assertion \<Delta> F A = {\<omega> |\<omega>. \<Delta> \<Turnstile> \<langle>A; \<omega>\<rangle> \<and> well_typed ((map_option (make_semantic_vtyp \<Delta>)) \<circ> F) (snd \<omega>)}"
+
+
+lemma rel_stable_assertion_make_semantic_assertionI :
+ "rel_stable_assertion \<omega> (make_semantic_assertion \<Delta> F A) = Stable ({\<omega>} \<otimes> make_semantic_assertion \<Delta> F A)"
+  by (simp add:rel_stable_assertion_def)
+
+fun compile :: "('a, 'a virtual_state) interp \<Rightarrow> (field_name \<rightharpoonup> vtyp) \<Rightarrow> stmt \<Rightarrow> ('a equi_state, 'a val, 'a custom) abs_stmt"
+  where
+  "compile \<Delta> F stmt.Skip = abs_stmt.Skip"
+
+| "compile \<Delta> F (stmt.If b C1 C2) = abs_stmt.If (make_semantic_bexp \<Delta> b) (compile \<Delta> F C1) (compile \<Delta> F C2)"
+| "compile \<Delta> F (stmt.Seq C1 C2) = abs_stmt.Seq (compile \<Delta> F C1) (compile \<Delta> F C2)"
+
+| "compile \<Delta> F (stmt.Havoc x) = abs_stmt.Havoc x"
+| "compile \<Delta> F (stmt.LocalAssign x e) = abs_stmt.LocalAssign x (make_semantic_exp \<Delta> e)"
+
+
+| "compile \<Delta> F (stmt.Inhale A) = abs_stmt.Inhale (make_semantic_assertion \<Delta> F A)"
+| "compile \<Delta> F (stmt.Exhale A) = abs_stmt.Exhale (make_semantic_assertion \<Delta> F A)"
+| "compile \<Delta> F (stmt.Assert A) = abs_stmt.Assert (make_semantic_assertion \<Delta> F A)"
+| "compile \<Delta> F (stmt.Assume A) = abs_stmt.Assume (make_semantic_assertion \<Delta> F A)"
+
+| "compile \<Delta> F (stmt.Unfold _ _ _) = abs_stmt.Skip"
+| "compile \<Delta> F (stmt.Fold _ _ _) = abs_stmt.Skip"
+| "compile \<Delta> F (stmt.Package _ _) = abs_stmt.Skip"
+| "compile \<Delta> F (stmt.Apply _ _) = abs_stmt.Skip"
+
+(* TODO: We can take the program as input, and emit the encodings *)
+| "compile \<Delta> F (stmt.MethodCall _ _ _) = undefined"
+| "compile \<Delta> F (stmt.While b I C) = undefined"
+| "compile \<Delta> F (stmt.Scope _ _) = undefined"
+
+| "compile \<Delta> F (stmt.FieldAssign r f e) = abs_stmt.Custom (FieldAssign (make_semantic_rexp \<Delta> r) f (make_semantic_exp \<Delta> e))"
+| "compile \<Delta> F (stmt.Label l) = abs_stmt.Custom (Label l)"
+
+
+
+
+
+(*
+definition viper_prog_verifies where
+  "viper_prog_verifies Pr \<Delta> ty C \<omega> \<longleftrightarrow> ConcreteSemantics.verifies ty (compile \<Delta> F C) \<omega>"
+  (* ty is a type-context *)
+*)
 
 
 
@@ -1198,11 +1217,6 @@ lemma make_semantic_assertion_inh :
   by (simp add:ConcreteSemantics.inh_def make_semantic_assertion_def)
 *)
 
-(*
-lemma rel_stable_assertion_make_semantic_assertionI :
- "rel_stable_assertion \<omega> (make_semantic_assertion \<Delta> F A) = Stable ({\<omega>} \<otimes> (\<langle>\<Delta>, F\<rangle> \<Turnstile> \<langle>A\<rangle>))"
-  by (simp add:rel_stable_assertion_def make_semantic_assertion_inh)
-*)
 
 section \<open>red_stmt with (overapproximating) postcondition\<close>
 
